src/tree/layer3/PruebaAbsurda.dfy
@@ -1,5 +1,259 @@
-include "layer1/KeyValue.dfy"
+include "../../../src/tree/layer1/UnorderedMap.dfy"
+include "../../../src/tree/layer1/OrderedSetUtils.dfy"
 
+
+
+
+
+
+trait OrderedMapIterator extends UnorderedMapIterator{
+
+function Traversed():set<K>
+    reads this, Parent(), Parent().Repr()
+    requires Valid()
+    requires Parent().Valid() 
+    ensures Traversed() <= (Parent().Model().Keys)
+    ensures forall x,y | x in Traversed() && y in Parent().Model().Keys-Traversed() :: x < y
+
+function method Peek():pairKV 
+    reads this, Parent(), Parent().Repr()
+    requires Valid()
+    requires Parent().Valid()
+    requires HasNext()
+    ensures Peek() in Parent().Model().Items &&
+            key(Peek()) !in Traversed() 
+    ensures key(Peek())==elemth(Parent().Model().Keys,|Traversed()|)  &&
+            value(Peek()) == Parent().Model()[key(Peek())]      
+    ensures forall k | k in Traversed() :: k < key(Peek())
+    ensures forall k | k in Parent().Model().Keys-Traversed()-{key(Peek())} :: key(Peek()) < k
+    ensures forall k | k in Parent().Model().Keys-Traversed() :: key(Peek()) <= k
+
+  
+
+ function method HasNext(): bool
+    reads this, Parent(), Parent().Repr()
+    requires Valid()
+    requires Parent().Valid()
+    ensures HasNext()  <==> Traversed() < Parent().Model().Keys && |Traversed()| < |Parent().Model().Keys|
+    //|Traversed()| < |Parent().Model()| es necesario para poder verificar con cota |s.Model()|-|it.Traversed()|
+    ensures !HasNext() ==> Traversed() == Parent().Model().Keys && |Traversed()| == |Parent().Model().Keys|
+  
+  function method Index(): int
+    reads this, Parent(), Parent().Repr()
+    requires Valid()
+    requires Parent().Valid()
+    ensures HasNext() ==> Index()==|Traversed()|==|smaller(Parent().Model().Keys,key(Peek()))|
+    ensures !HasNext() ==> Index()==|Parent().Model()|
+  
+
+  method Next() returns (p: pairKV)
+    modifies this
+    requires Valid()
+    requires Parent().Valid()
+    requires HasNext()
+    requires allocated(Parent())
+    requires forall it | it in Parent().Repr() :: allocated(it)
+    ensures Parent().Valid()
+    ensures Valid()
+    ensures old(Parent()) == Parent()
+    ensures old(Parent().Model()) == Parent().Model()
+
+    ensures forall x {:trigger x in Parent().Repr(), x in old(Parent().Repr())} | x in Parent().Repr() - old(Parent().Repr()) :: fresh(x)
+    ensures fresh(Parent().Repr()-old(Parent().Repr()))
+    ensures forall x | x in Parent().Repr() :: allocated(x)
+
+    ensures Parent().Iterators() == old(Parent().Iterators())
+
+    ensures p==old(Peek()) && Traversed() == {old(key(Peek()))}+old(Traversed())
+    ensures |Traversed()|==1+|old(Traversed())|
+    ensures HasNext() ==> key(Peek())==elemth(Parent().Model().Keys,|Traversed()|)//already known
+
+    ensures forall it | it in Parent().Iterators() && old(it.Valid()) ::
+      it.Valid() && (it != this ==> it.Traversed() == old(it.Traversed()) && (it.HasNext() ==> it.Peek()==old(it.Peek())))
+
+function method HasPrev(): bool//igual que HasNext
+    reads this, Parent(), Parent().Repr()
+    requires Valid()
+    requires Parent().Valid()
+    ensures HasPrev()  <==> Traversed() < Parent().Model().Keys && |Traversed()| < |Parent().Model().Keys|
+    //|Traversed()| < |Parent().Model()| es necesario para poder verificar con cota |s.Model()|-|it.Traversed()|
+    ensures !HasPrev() ==> Traversed() == Parent().Model().Keys && |Traversed()| == |Parent().Model().Keys|
+  
+
+  method Prev() returns (p: pairKV)
+    modifies this
+    requires Valid()
+    requires Parent().Valid()
+    requires HasNext() 
+    requires allocated(Parent())
+    requires forall it | it in Parent().Repr() :: allocated(it)
+    ensures Parent().Valid()
+    ensures Valid()
+    ensures old(Parent()) == Parent()
+    ensures old(Parent().Model()) == Parent().Model()
+
+    ensures forall x {:trigger x in Parent().Repr(), x in old(Parent().Repr())} | x in Parent().Repr() - old(Parent().Repr()) :: fresh(x)
+    ensures fresh(Parent().Repr()-old(Parent().Repr()))
+    ensures forall x | x in Parent().Repr() :: allocated(x)
+
+    ensures Parent().Iterators() == old(Parent().Iterators())
+    ensures p==old(Peek())  
+    ensures old(Traversed())=={} ==> Traversed()==Parent().Model().Keys
+    ensures old(Traversed())!={} ==> (Traversed()==old(Traversed())-{maximum(old(Traversed()))} &&
+                                      (HasNext() ==> key(Peek())==maximum(old(Traversed()))))
+    ensures forall it | it in Parent().Iterators() && old(it.Valid()) ::
+      it.Valid() && (it != this ==> it.Traversed() == old(it.Traversed()) && (it.HasNext() ==> it.Peek()==old(it.Peek())))
+
+  method Copy() returns (it: UnorderedMapIterator)
+    modifies Parent(), Parent().Repr()
+    requires Valid()
+    requires Parent().Valid()
+    requires allocated(Parent())
+    requires forall it | it in Parent().Iterators() :: allocated(it)
+    ensures fresh(it)
+    ensures Valid()
+    ensures Parent() == old(Parent())
+    ensures Parent().Valid()
+    ensures Parent().Model() == old(Parent().Model())
+
+    ensures forall x {:trigger x in Parent().Repr(), x in old(Parent().Repr())} | x in Parent().Repr() - old(Parent().Repr()) :: fresh(x)
+    ensures fresh(Parent().Repr()-old(Parent().Repr()))
+    ensures forall x | x in Parent().Repr() :: allocated(x)
+    
+    ensures it is OrderedMapIterator
+    ensures it.Valid()
+    ensures Parent().Iterators() == {it} + old(Parent().Iterators())
+    ensures Parent() == it.Parent()
+
+    ensures Traversed() == it.Traversed() 
+    ensures HasNext() ==> Peek()==it.Peek()
+    ensures forall it | it in old(Parent().Iterators()) && old(it.Valid()) ::
+      it.Valid() && it.Traversed() == old(it.Traversed()) && (it.HasNext() ==> it.Peek()==old(it.Peek()))
+
+
+}
+
+trait OrderedMap extends UnorderedMap {
+  
+ 
+ function Iterators(): set<UnorderedMapIterator>
+    reads this, Repr()
+    requires Valid()
+    ensures forall it | it in Iterators() :: it in Repr() && it.Parent() == this
+    ensures forall it | it in Iterators() :: it is OrderedMapIterator
+
+method First() returns (it: UnorderedMapIterator)
+    modifies this, Repr()
+    requires Valid()
+    requires forall x | x in Repr() :: allocated(x)
+    ensures Valid()
+    ensures Model() == old(Model())
+
+    ensures forall x {:trigger x in Repr(), x in old(Repr())} | x in Repr() - old(Repr()) :: fresh(x)
+    ensures fresh(Repr()-old(Repr()))
+    ensures forall x | x in Repr() :: allocated(x)
+
+    ensures it is OrderedMapIterator
+    ensures fresh(it)
+    ensures Iterators() == {it} + old(Iterators())
+    ensures it.Valid()
+    ensures it.Parent() == this
+    ensures it.Traversed()=={} 
+    ensures Model()!=map[] ==> it.HasNext() && key(it.Peek())==elemth(Model().Keys,0)
+    ensures forall it | it in old(Iterators()) && old(it.Valid()) ::
+      it.Valid() && it.Traversed() == old(it.Traversed()) && (it.HasNext() ==> it.Peek()==old(it.Peek()))
+
+  method Last() returns (it: OrderedMapIterator)//iterator to the last element
+    modifies this, Repr()
+    requires Valid()
+    requires forall x | x in Repr() :: allocated(x)
+    ensures Valid()
+    ensures Model() == old(Model())
+
+    ensures forall x {:trigger x in Repr(), x in old(Repr())} | x in Repr() - old(Repr()) :: fresh(x)
+    ensures fresh(Repr()-old(Repr()))
+    ensures forall x | x in Repr() :: allocated(x)
+
+    ensures fresh(it)
+    ensures Iterators() == {it} + old(Iterators())
+    ensures it.Valid()
+    ensures it.Parent() == this
+    ensures Model()!=map[] ==> it.HasNext() && it.Traversed()==Model().Keys-{elemth(Model().Keys,|Model().Keys|-1)} && key(it.Peek())==elemth(Model().Keys,|Model().Keys|-1)
+    ensures Model()==map[] ==> it.Traversed()=={}
+    ensures forall it | it in old(Iterators()) && old(it.Valid()) ::
+      it.Valid() && it.Traversed() == old(it.Traversed()) && (it.HasNext() ==> it.Peek()==old(it.Peek()))
+
+
+
+
+method find(k:K) returns (newt:UnorderedMapIterator)
+    modifies this, Repr()
+    requires Valid()
+    requires forall x | x in Repr() :: allocated(x)
+    ensures Valid() 
+    ensures Model()==old(Model())
+    
+    ensures newt is OrderedMapIterator
+    ensures fresh(newt) 
+    ensures newt.Valid() && newt.Parent()==this
+    ensures k in old(Model()) ==> newt.HasNext() && key(newt.Peek())==k
+    ensures k !in old(Model()) ==> newt.Traversed()==Model().Keys
+
+    ensures forall x {:trigger x in Repr(), x in old(Repr())} | x in Repr() - old(Repr()) :: fresh(x)
+    ensures fresh(Repr()-old(Repr()))
+    ensures forall x | x in Repr() :: allocated(x)
+
+    ensures Iterators() == {newt}+old(Iterators())
+
+  method insert(mid: UnorderedMapIterator, k: K, v : V) returns (newt:UnorderedMapIterator)
+    modifies this, Repr()
+    requires Valid()
+    requires mid.Valid() 
+    requires mid.Parent() == this
+    requires mid in Iterators()
+    requires forall x | x in Repr() :: allocated(x)
+    ensures Valid()
+    ensures Model() == old(Model())[k:=v]
+
+    ensures newt is OrderedMapIterator
+    ensures fresh(newt)
+    ensures Iterators() == {newt}+old(Iterators())
+    ensures newt.Valid() && newt.Parent()==this  
+    ensures newt.HasNext() && newt.Peek()==(k,v) && newt.Traversed()==smaller(Model().Keys,k)
+
+    ensures forall x {:trigger x in Repr(), x in old(Repr())} | x in Repr() - old(Repr()) :: fresh(x)
+    ensures fresh(Repr()-old(Repr()))
+    ensures forall x | x in Repr() :: allocated(x)
+
+    //points either to the inserted elemento or to the already existing one
+ 
+
+
+
+  method erase(mid:UnorderedMapIterator) returns (next: UnorderedMapIterator)
+    modifies this, Repr()
+    requires Valid()
+    requires mid.Valid()
+    requires mid.Parent() == this
+    requires mid.HasNext()
+    requires mid in Iterators()
+    requires forall x | x in Repr() :: allocated(x)
+    ensures Valid()
+    ensures Model()== map k | k in old(Model()) && k!=old(key(mid.Peek()))::old(Model())[k]
+    
+    ensures next is OrderedMapIterator
+    ensures fresh(next)
+    ensures Iterators() == {next}+old(Iterators())
+    ensures next.Valid() && next.Parent()==this 
+    ensures next.Traversed()==old(mid.Traversed()) &&
+                (next.HasNext() ==> key(next.Peek())==elemth(Model().Keys,|next.Traversed()|) && value(next.Peek())==Model()[key(next.Peek())])
+
+
+    ensures forall x {:trigger x in Repr(), x in old(Repr())} | x in Repr() - old(Repr()) :: fresh(x)
+    ensures fresh(Repr()-old(Repr()))
+    ensures forall x | x in Repr() :: allocated(x)
+ 
+}
 
 datatype tree<A> = Empty | Node(left: tree<A>, data: A, right: tree<A>)
  
@@ -91,6 +345,8 @@ function method depth<A>(t: tree<A>): nat
 
 datatype Color = Red | Black
 
+type K = int
+type V = int
 
 class TNode {
   var key: K;
@@ -343,34 +599,7 @@ class Tree {
     }
   }
 
-lemma ModelRelationWithSkeletonKeys(k: K)
-requires Valid() 
-requires SearchTree()
-ensures (set n | n in elems(skeleton) && n.key < k :: n.key) == 
-        (set m | m in MapModel() && m < k) 
-ensures (set n | n in elems(skeleton) && n.key > k :: n.key) == 
-        (set m | m in MapModel() && m > k) 
-ensures |(set n | n in elems(skeleton) && n.key < k :: n.key)| == 
-        |(set m | m in MapModel() && m < k)| 
-ensures |(set n | n in elems(skeleton) && n.key > k :: n.key)| == 
-        |(set m | m in MapModel() && m > k)| 
-         
 
-{ assert (set n | n in elems(skeleton) && n.key < k :: n.key) <=
-        (set m | m in MapModel() && m < k); 
-  forall m | m in MapModel() && m < k 
-  ensures m in (set n | n in elems(skeleton) && n.key < k :: n.key)
-  {ModelRelationWithSkeletonKey(m);
-   assert exists n | n in elems(skeleton) :: n.key == m < k;
-  }
- forall m | m in MapModel() && m > k 
-  ensures m in (set n | n in elems(skeleton) && n.key > k :: n.key)
-  {ModelRelationWithSkeletonKey(m);
-   assert exists n | n in elems(skeleton) :: n.key == m > k;
-
-  }
-  
-}
   function method isEmpty(): bool
     reads this, Repr()
     requires Valid()
@@ -933,39 +1162,6 @@ ensures MapModelRec(newSk)==moSk-{node.key}
     root, skeleton, removedNode := RemoveRec(root, skeleton, k);
   }
 
-static function LeftPathAux(n: TNode, sk: tree<TNode>): seq<TNode>
-    reads elems(sk)
-    requires SearchTreeRec(sk)
-    requires n in elems(sk)
-  {
-     match sk {
-       case Node(l, x, r) => 
-          if n == x then
-            [n]
-          else if n.key < x.key then
-            LeftPathAux(n, l) + [x]
-          else
-            LeftPathAux(n, r)
-    }
-  }
+
   
-  lemma mapModelRecContained(node:TNode,sk:tree<TNode>,node':TNode,sk':tree<TNode>)
-  requires ValidRec(node,sk) && ValidRec(node',sk')
-  requires SearchTreeRec(sk) && SearchTreeRec(sk')
-  requires elems(sk) <= elems(sk')
-  ensures MapModelRec(sk).Items <= MapModelRec(sk').Items
-{
-  if (MapModelRec(sk).Items!={})
-   { forall p | p in MapModelRec(sk).Items
-     ensures p in MapModelRec(sk').Items
-   {
-     ModelRelationWithSkeletonRecR(node,sk,p.0,p.1);
-    var n :| n in elems(sk) && n.key == p.0 && n.value == p.1;
-    assert n in elems(sk');
-    ModelRelationWithSkeletonRecL(node',sk',p.0,p.1);
-    assert p.0 in MapModelRec(sk') && MapModelRec(sk')[p.0]==p.1;
-    assert p in MapModelRec(sk').Items;}
-  }
-  else{}
-}
 }
