src/tree/layer1/KeyValue.dfy
@@ -1,0 +1,9 @@
+type K = int
+type V = int
+type pairKV = (K,V)
+
+function key(p:pairKV):K
+{p.0}
+
+function value(p:pairKV):V
+{p.1}
